new_proof/RDInv3.v
@@ -64,8 +64,8 @@ Proof.
   apply empty_basic_typing_arrow_value_lam_exists. refinement_solver.
 Qed.
 
-Lemma is_arr_open_trans: forall τ_x (v2: value),
-  is_arr τ_x -> is_arr (τ_x ^r^ v2).
+Lemma is_arr_open_trans: forall τ_x k (v2: value),
+  is_arr τ_x -> is_arr ({k ~r> v2} τ_x).
 Proof.
   intros. destruct τ_x; auto.
 Qed.
@@ -76,32 +76,6 @@ Ltac wf_regular_solver :=
   match goal with
   | [H: wf_ctxrR ?st ?Γ |- ok_dctx _ ?Γ] => apply wf_ctxrR_regular1 in H; auto
   end.
-
-Ltac lc_simpl4 :=
-  match goal with
-  | [H: context [{?x := ?v }t ({_ ~t> (vfvar ?x)} ?e)] |- _ ] =>
-      assert (x ∉ stale e) as Htmp by fast_set_solver;
-      rewrite open_subst_same_tm in H; auto; try clear Htmp
-  | [|- context [{?x := ?v }t ({_ ~t> (vfvar ?x)} ?e)]] =>
-      assert (x ∉ stale e) as Htmp by fast_set_solver;
-      rewrite open_subst_same_tm; auto; try clear Htmp
-  | [H: context [{?x := ?v }v ({_ ~v> (vfvar ?x)} ?e)] |- _ ] =>
-      assert (x ∉ stale e) as Htmp by fast_set_solver;
-      rewrite open_subst_same_value in H; auto; try clear Htmp
-  | [|- context [{?x := ?v }v ({_ ~v> (vfvar ?x)} ?e)]] =>
-      assert (x ∉ stale e) as Htmp by fast_set_solver;
-      rewrite open_subst_same_value; auto; try clear Htmp
-  end.
-
-Lemma tletapp_typable
-     : ∀ Γ (v1 v2 : value) (e : tm) (x : atom) (T1 T2 T: ty),
-         x ∉ fv_tm e -> Γ ⊢t v1 ⋮v (T2 ⤍ T1) -> Γ ⊢t v2 ⋮v T2
-         → (Γ ++ [(x, T1)]) ⊢t e ^t^ x ⋮t T -> Γ ⊢t tletapp v1 v2 e ⋮t T.
-Proof.
-  intros. auto_exists_L; intros.
-  apply basic_has_type_renaming with (x0:=x0) in H2; auto.
-  lc_simpl4. fast_set_solver. basic_typing_solver.
-Qed.
 
 Ltac inv_rd_simpl3 :=
   repeat match goal with
@@ -119,20 +93,13 @@ Ltac inv_rd_simpl3 :=
 
 Ltac auto_ty_exfalso5 :=
   match goal with
-  | [H: is_arr ?τ_x, H': {v:_|_|_|_} = ?τ_x ^r^ ?v2 |- _ ] =>
-      assert (is_arr (τ_x ^r^ v2)) as Htmp by auto;
+  | [H: is_arr ?τ_x, H': {v:_|_|_|_} = {?k ~r> ?v2} ?τ_x |- _ ] =>
+      assert (is_arr ({k ~r> v2} τ_x)) as Htmp by auto;
       rewrite <- H' in Htmp; auto_ty_exfalso2
-  | [H: is_arr ?τ_x, H': [v:_|_|_|_] = ?τ_x ^r^ ?v2 |- _ ] =>
-      assert (is_arr (τ_x ^r^ v2)) as Htmp by auto;
+  | [H: is_arr ?τ_x, H': [v:_|_|_|_] = {?k ~r> ?v2} ?τ_x |- _ ] =>
+      assert (is_arr ({k ~r> v2} τ_x)) as Htmp by auto;
       rewrite <- H' in Htmp; auto_ty_exfalso2
   end.
-
-Ltac instantiation_simp :=
-   repeat match goal with
-    | [H: instantiation [] _ |- _ ] => invclear H
-    | [H: context [tm_msubst [] _ ] |- _ ] => simpl in H
-    | [|- context [tm_msubst [] _ ] ] => simpl
-    end.
 
 Lemma rR_open_trans_empty': forall τ st (c: constant) e,
     {1;<b[↦c]> b∅;st}⟦τ⟧ e -> ({0;b∅;st}⟦τ ^r^ c⟧) e.
@@ -161,183 +128,11 @@ Proof.
     apply H in H4. mydestr. auto_reduction_exfalso1.
 Qed.
 
-Lemma tm_open_then_msubst_k: forall Γ env,
-    instantiation Γ env ->
-    (forall e k v, tm_msubst env ({k ~t> v} e) = ({k ~t> (value_msubst env v)} (tm_msubst env e))).
-Proof.
-  intros Γ env Hi; induction Hi; simpl; intros; auto.
-  rewrite subst_open_tm; basic_typing_solver6.
-Qed.
-
-Lemma mk_app_v_v_reduce_to_letapp:
-  ∀ (Γ : listctx ty) (Tx T2 : ty) (v1 v2 : value),
-    Γ ⊢t v2 ⋮v Tx -> Γ ⊢t v1 ⋮v (Tx ⤍ T2) ->
-    (mk_app v1 v2) <-<{ Γ; T2} (tletapp v1 v2 (vbvar 0)).
-Proof.
-  intros. constructor.
-  - eapply mk_app_typable; eauto.
-  - auto_exists_L; simpl; intros. basic_typing_vfavr_solver.
-  - unfold termRraw. intros Γv. intros. unfold mk_app in H2. reduction_simpl1.
-    rewrite lete_step_spec in H2; simpl; mydestr. simpl in H4. reduction_simpl1.
-    rewrite lete_step_spec in H4; simpl; mydestr. simpl in H6. reduction_simpl1.
-Qed.
-
-Lemma mk_app_v_v_reduce_to_letapp':
-  ∀ (Γ : listctx ty) (Tx T2 : ty) (v1 v2 : value),
-    Γ ⊢t v2 ⋮v Tx -> Γ ⊢t v1 ⋮v (Tx ⤍ T2) ->
-    (tletapp v1 v2 (vbvar 0)) <-<{ Γ; T2} (mk_app v1 v2).
-Proof.
-  intros. constructor.
-  - auto_exists_L; simpl; intros. basic_typing_vfavr_solver.
-  - eapply mk_app_typable; eauto.
-  - unfold termRraw. intros Γv. intros. unfold mk_app. reduction_simpl1.
-    rewrite lete_step_spec. split; auto. apply mk_app_body. reduction_solver1.
-    exists (value_msubst Γv v1). split; eauto. reduction_solver1.
-    simpl. reduction_simpl1.
-    rewrite lete_step_spec. split; auto. reduction_solver1. reduction_simpl1.
-    exists (value_msubst Γv v2). split; eauto. reduction_solver1. reduction_simpl1.
-Qed.
-
-(* Lemma mk_app_v_v_reduce_to_letapp_e: *)
-(*   ∀ (Γ : listctx ty) (Tx T2 T: ty) (v1 v2 : value) e, *)
-(*     Γ ⊢t v2 ⋮v Tx -> Γ ⊢t v1 ⋮v (Tx ⤍ T2) -> *)
-(*     (exists (L: aset), ∀ x : atom, x ∉ L → (Γ ++ [(x, T2)]) ⊢t e ^t^ x ⋮t T) -> *)
-(*     (tlete (mk_app v1 v2) e) <-<{ Γ; T} (tletapp v1 v2 e). *)
-(* Proof. *)
-(*   intros. constructor. *)
-(*   - mydestr. econstructor; eauto. eapply mk_app_typable; eauto. *)
-(*   - mydestr. econstructor; eauto. *)
-(*   - unfold termRraw. intros Γv. intros. unfold mk_app in H3. reduction_simpl1. *)
-(*     rewrite lete_step_spec in H3; simpl; mydestr. simpl in H4. reduction_simpl1. *)
-(*     rewrite lete_step_spec in H4; simpl; mydestr. simpl in H7. reduction_simpl1. *)
-(*     rewrite lete_step_spec in H7; simpl; mydestr. simpl in H9. reduction_simpl1. *)
-(*     reduction_simpl1. *)
-(* Qed. *)
-
-Lemma lete_0_reduce_to_self_aux: ∀ (Γ : listctx ty) e,
-    termRraw Γ e (tlete e (vbvar 0)).
-Proof.
-  intros. unfold termRraw. intros Γv. intros. reduction_simpl1.
-  rewrite lete_step_spec. split; auto. eexists; split; eauto. reduction_solver1.
-Qed.
-
-Lemma lete_0_reduce_to_self_aux': ∀ (Γ : listctx ty) e,
-    termRraw Γ (tlete e (vbvar 0)) e.
-Proof.
-  intros. unfold termRraw. intros Γv. intros. reduction_simpl1.
-  rewrite lete_step_spec in H0; mydestr. simpl in H2. reduction_simpl1; auto.
-Qed.
-
-Lemma lete_0_reduce_to_self: ∀ (Γ : listctx ty) (T : ty) e,
-    Γ ⊢t e ⋮t T -> e <-<{ Γ; T} (tlete e (vbvar 0)).
-Proof.
-  intros. constructor; auto.
-  - auto_exists_L; simpl; intros. basic_typing_vfavr_solver.
-  - unfold termRraw. intros Γv. intros. reduction_simpl1.
-     rewrite lete_step_spec. split; auto. eexists; split; eauto. reduction_solver1.
-Qed.
-
-Lemma lete_0_reduce_to_self': ∀ (Γ : listctx ty) (T : ty) e,
-    Γ ⊢t e ⋮t T -> (tlete e (vbvar 0)) <-<{ Γ; T} e.
-Proof.
-  intros. constructor; auto.
-  - auto_exists_L; simpl; intros. basic_typing_vfavr_solver.
-  - unfold termRraw. intros Γv. intros. reduction_simpl1.
-    rewrite lete_step_spec in H1; mydestr. simpl in H3. reduction_simpl1; auto.
-Qed.
-
-(* Lemma basic_typing_implies_open_value: forall Γ (T1 T2: ty) (v1: value) (e2: value), *)
-(*     Γ ⊢t v1 ⋮v T1 -> Γ ⊢t e2 ⋮v T1 ⤍ T2 -> Γ ⊢t (e2 ^v^ v1) ⋮v T2. *)
-(* Proof. *)
-(*   intros. invclear H0. *)
-
-Lemma vfix_implies_open_tyable:
-  ∀ (Γ : context) (v1 : value) (Tx T : ty),
-    Γ ⊢t vfix (Tx ⤍ T) v1 ⋮v Tx ⤍ T → Γ ⊢t v1 ^v^ (vfix (Tx ⤍ T) v1) ⋮v Tx ⤍ T.
-Proof.
-  intros. invclear H. auto_pose_fv f.
-  assert ((Γ ++ [(f, Tx0 ⤍ T)]) ⊢t (vlam Tx0 e) ^t^ f ⋮t (Tx0 ⤍ T)) by fast_set_solver.
-  invclear H0.
-  apply basic_typing_subst_value_pre with (u:=(vfix (Tx0 ⤍ T) (vlam Tx0 e))) in H4; eauto.
-  simpl in H4. simpl. lc_simpl4.
-Qed.
-
-Lemma letapp_fix_reduce_to_open:
-  ∀ (Γ : listctx ty) (Tx T2 : ty) e1 (v2 : value),
-    Γ ⊢t v2 ⋮v Tx -> Γ ⊢t (vfix (Tx ⤍ T2) (vlam Tx e1)) ⋮v (Tx ⤍ T2) ->
-    (tletapp (vfix (Tx ⤍ T2) (vlam Tx e1)) v2 (vbvar 0)) <-<{ Γ; T2}
-      (({1 ~t> (vfix (Tx ⤍ T2) (vlam Tx e1))} e1) ^t^ v2).
-Proof.
-  intros. constructor.
-  - auto_exists_L; simpl; intros. basic_typing_vfavr_solver.
-  - apply vfix_implies_open_tyable in H0. simpl in H0.
-    apply vlam_implies_open_tyable with (v2:= v2) in H0; auto.
-  - unfold termRraw. intros Γv. intros. unfold mk_app in H2. msubst_simpl.
-    rewrite letapp_step_spec in H2; mydestr. destruct H5; mydestr; subst; invclear H5. simpl in H6.
-    rewrite letapp_step_spec in H6; mydestr. destruct H8; mydestr; subst; invclear H8. simpl in H9.
-    eapply lete_0_reduce_to_self_aux'; eauto. msubst_simpl.
-    setoid_rewrite tm_open_then_msubst_k; eauto.
-    setoid_rewrite tm_open_then_msubst_k; eauto. msubst_simpl. auto.
-Qed.
-
-Lemma letapp_fix_reduce_to_open':
-  ∀ (Γ : listctx ty) (Tx T2 : ty) e1 (v2 : value),
-    Γ ⊢t v2 ⋮v Tx -> Γ ⊢t (vfix (Tx ⤍ T2) (vlam Tx e1)) ⋮v (Tx ⤍ T2) ->
-    (({1 ~t> (vfix (Tx ⤍ T2) (vlam Tx e1))} e1) ^t^ v2) <-<{ Γ; T2} (tletapp (vfix (Tx ⤍ T2) (vlam Tx e1)) v2 (vbvar 0)).
-Proof.
-  intros. constructor.
-  - apply vfix_implies_open_tyable in H0. simpl in H0.
-    apply vlam_implies_open_tyable with (v2:= v2) in H0; auto.
-  - auto_exists_L; simpl; intros. basic_typing_vfavr_solver.
-  - unfold termRraw. intros Γv. intros. msubst_simpl.
-    rewrite letapp_step_spec. repeat split; auto.
-    { assert (lc (vfix (Tx ⤍ T2) (vlam Tx e1))). basic_typing_solver.
-      assert (lc (value_msubst Γv (vfix (Tx ⤍ T2) (vlam Tx e1)))).
-      eapply instantiation_implies_value_msubst_lc; eauto. msubst_simpl. auto. }
-    reduction_solver1.
-    right. do 2 eexists; split; eauto. simpl.
-    rewrite letapp_step_spec. repeat split; auto.
-    { apply vfix_implies_open_tyable in H0. simpl in H0.
-      assert (lc (vlam Tx ({1 ~t> vfix (Tx ⤍ T2) (vlam Tx e1)} e1))). basic_typing_solver.
-      eapply instantiation_implies_value_msubst_lc in H3; eauto. msubst_simpl.
-      setoid_rewrite tm_open_then_msubst_k in H3; eauto. msubst_simpl. auto. }
-    reduction_solver1.
-    left. do 2 eexists; split; eauto. simpl.
-    eapply lete_0_reduce_to_self_aux in H2; eauto. msubst_simpl.
-    setoid_rewrite tm_open_then_msubst_k in H2; eauto.
-    setoid_rewrite tm_open_then_msubst_k in H2; eauto. msubst_simpl. auto.
-Qed.
-
-Lemma termR_trans_better:
-  ∀ (Γ : context) (T : ty) (e1 e2 e3 : tm),
-    e1 <-<{ Γ; T} e2 → e2 <-<{ Γ; T} e3 → e1 <-<{ Γ; T} e3.
-Proof.
-  intros. eapply termR_trans; eauto.
-  - invclear H; auto.
-  - invclear H; auto.
-  - invclear H0; auto.
-Qed.
-
-Lemma mk_app_reduce_to_open_fix:
-  ∀ (Γ : listctx ty) (Tx T2 : ty) e1 (v2 : value),
-    Γ ⊢t v2 ⋮v Tx -> Γ ⊢t (vfix (Tx ⤍ T2) (vlam Tx e1)) ⋮v (Tx ⤍ T2) ->
-    (mk_app (vfix (Tx ⤍ T2) (vlam Tx e1)) v2) <-<{ Γ; T2}
-      (({1 ~t> (vfix (Tx ⤍ T2) (vlam Tx e1))} e1) ^t^ v2).
-Proof.
-  intros. apply termR_trans_better with (e2:= tletapp (vfix (Tx ⤍ T2) (vlam Tx e1)) v2 (vbvar 0)).
-  - eapply mk_app_v_v_reduce_to_letapp; eauto.
-  - eapply letapp_fix_reduce_to_open; eauto.
-Qed.
-
-Lemma mk_app_reduce_to_open_fix':
-  ∀ (Γ : listctx ty) (Tx T2 : ty) e1 (v2 : value),
-    Γ ⊢t v2 ⋮v Tx -> Γ ⊢t (vfix (Tx ⤍ T2) (vlam Tx e1)) ⋮v (Tx ⤍ T2) ->
-     (({1 ~t> (vfix (Tx ⤍ T2) (vlam Tx e1))} e1) ^t^ v2) <-<{ Γ; T2} (mk_app (vfix (Tx ⤍ T2) (vlam Tx e1)) v2).
-Proof.
-  intros. apply termR_trans_better with (e2:= tletapp (vfix (Tx ⤍ T2) (vlam Tx e1)) v2 (vbvar 0)).
-  - eapply letapp_fix_reduce_to_open'; eauto.
-  - eapply mk_app_v_v_reduce_to_letapp'; eauto.
-Qed.
+Ltac reduction_simpl0 :=
+  repeat match goal with
+  | [H: tvalue _ ↪* tvalue _ |- _ ] =>
+      rewrite value_reduce_to_value_implies_same in H; mydestr; subst
+  end.
 
 Lemma rR_letapp_overbase_underbase:
   forall st τ_x (v1: value) (c2: constant) b1 n1 d1 ϕ1 b2 n2 d2 ϕ2,
@@ -345,40 +140,25 @@ Lemma rR_letapp_overbase_underbase:
   (∀ e_wf : tm, ({0;b∅;st}⟦[v:b1|n1|d1|ϕ1]⟧) e_wf → ∃ v_wf : value, e_wf ↪* v_wf) ->
   ({0;b∅;st}⟦[v:b1|n1|d1|ϕ1]⟧) c2 ->
   ({0;b∅;st}⟦-:{v:b1|n1|d1|ϕ1}⤑ τ_x⟧) v1 ->
-  (exists e1, ({0;b∅;st}⟦ τ_x ^r^ c2 ⟧) (e1 ^t^ c2) /\ (e1 ^t^ c2) <-<{ []; b2} (mk_app v1 c2)).
+  (exists e1, ({0;b∅;st}⟦ τ_x ^r^ c2 ⟧) e1 /\ e1 <-<{ []; b2} (mk_app v1 c2)).
 Proof.
   intros; subst.
   assert (ϕ1 b∅ st c2 /\ [] ⊢t c2 ⋮v b1) as (Hz & HzT). eapply wf_implies_base_phi_sat; eauto.
   destruct (rR_arrow_value_lam_exists_oarr _ _ _ _ _ _ _ _ _ H2); mydestr; subst.
-  - rename x into e1. exists e1. split.
-    + invclear H2; invclear H1; mydestr. apply H5 in Hz; auto.
+  - rename x into e1. exists (e1 ^t^ c2). split.
+    + invclear H2; invclear H1; mydestr. reduction_simpl0.
+      apply H6 in Hz; auto.
       apply rR_open_trans_empty' in Hz; auto.
       eapply termR_perserve_rR; eauto. refinement_solver. simpl.
       apply mk_app_reduce_to_open; auto. basic_typing_solver.
     + apply mk_app_reduce_to_open'; auto. refinement_solver.
-  - rename x into e1. exists (({1 ~t> (vfix (b1 ⤍ b2) (vlam b1 e1))} e1)). split.
-    + invclear H2; invclear H1; mydestr. apply H5 in Hz; auto.
+  - rename x into e1. exists (({1 ~t> c2} e1) ^t^ (vfix (b1 ⤍ b2) (vlam b1 e1))). split.
+    + invclear H2; invclear H1; mydestr. reduction_simpl0. apply H6 in Hz; auto.
       apply rR_open_trans_empty' in Hz; auto.
       eapply termR_perserve_rR; eauto. refinement_solver. simpl.
       apply mk_app_reduce_to_open_fix; auto. refinement_solver.
     + apply mk_app_reduce_to_open_fix'; auto. refinement_solver.
 Qed.
-
-(* Lemma rR_letapp_overbase_underbase_lam: *)
-(*   forall st τ_x e1 (c2: constant) b1 n1 d1 ϕ1 b2 n2 d2 ϕ2, *)
-(*   τ_x = [v:b2|n2|d2|ϕ2] -> *)
-(*   (∀ e_wf : tm, ({0;b∅;st}⟦[v:b1|n1|d1|ϕ1]⟧) e_wf → ∃ v_wf : value, e_wf ↪* v_wf) -> *)
-(*   ({0;b∅;st}⟦[v:b1|n1|d1|ϕ1]⟧) c2 -> *)
-(*   ({0;b∅;st}⟦-:{v:b1|n1|d1|ϕ1}⤑ τ_x⟧) (vlam b1 e1) -> *)
-(*   ({0;b∅;st}⟦ τ_x ^r^ c2 ⟧) (e1 ^t^ c2). *)
-(* Proof. *)
-(*   intros; subst. *)
-(*   assert (ϕ1 b∅ st c2 /\ [] ⊢t c2 ⋮v b1) as (Hz & HzT). eapply wf_implies_base_phi_sat; eauto. *)
-(*   - invclear H2; invclear H1; mydestr. apply H5 in Hz; auto. *)
-(*     apply rR_open_trans_empty' in Hz; auto. *)
-(*     eapply termR_perserve_rR; eauto. refinement_solver. simpl. *)
-(*     apply mk_app_reduce_to_open; auto. basic_typing_solver. *)
-(* Qed. *)
 
 Lemma rR_letapp_overbase_lam:
   forall st τ_x e1 (c2: constant) b1 n1 d1 ϕ1,
@@ -389,7 +169,7 @@ Lemma rR_letapp_overbase_lam:
 Proof.
   intros; subst.
   assert (ϕ1 b∅ st c2 /\ [] ⊢t c2 ⋮v b1) as (Hz & HzT). eapply wf_implies_base_phi_sat; eauto.
-  invclear H0; invclear H1; mydestr. apply H4 in Hz; auto.
+  invclear H0; invclear H1; mydestr. reduction_simpl0. apply H6 in Hz; auto.
   apply rR_open_trans_empty' in Hz; auto.
   eapply termR_perserve_rR; eauto. refinement_solver. refinement_solver.
   apply mk_app_reduce_to_open; auto.
@@ -401,32 +181,16 @@ Lemma rR_letapp_overbase_fix:
   (∀ e_wf : tm, ({0;b∅;st}⟦[v:b1|n1|d1|ϕ1]⟧) e_wf → ∃ v_wf : value, e_wf ↪* v_wf) ->
   ({0;b∅;st}⟦[v:b1|n1|d1|ϕ1]⟧) c2 ->
   ({0;b∅;st}⟦-:{v:b1|n1|d1|ϕ1}⤑ τ_x⟧) (vfix (b1 ⤍ ⌊ τ_x ⌋ ) (vlam b1 e1)) ->
-  ({0;b∅;st}⟦ τ_x ^r^ c2 ⟧) (({1 ~t> (vfix (b1 ⤍ ⌊ τ_x ⌋) (vlam b1 e1))} e1) ^t^ c2).
+  ({0;b∅;st}⟦ τ_x ^r^ c2 ⟧) (({1 ~t> c2} e1) ^t^ (vfix (b1 ⤍ ⌊ τ_x ⌋) (vlam b1 e1))).
 Proof.
   intros; subst.
   assert (ϕ1 b∅ st c2 /\ [] ⊢t c2 ⋮v b1) as (Hz & HzT). eapply wf_implies_base_phi_sat; eauto.
-  invclear H0; invclear H1; mydestr. apply H4 in Hz; auto.
+  invclear H0; invclear H1; mydestr. reduction_simpl0. apply H6 in Hz; auto.
   apply rR_open_trans_empty' in Hz; auto.
   eapply termR_perserve_rR; eauto. refinement_solver. refinement_solver.
   inv_rd_simpl1.
   apply mk_app_reduce_to_open_fix; auto.
 Qed.
-
-(* Lemma rR_letapp_overbase_underbase_fix: *)
-(*   forall st τ_x e1 (c2: constant) b1 n1 d1 ϕ1 b2 n2 d2 ϕ2, *)
-(*   τ_x = [v:b2|n2|d2|ϕ2] -> *)
-(*   (∀ e_wf : tm, ({0;b∅;st}⟦[v:b1|n1|d1|ϕ1]⟧) e_wf → ∃ v_wf : value, e_wf ↪* v_wf) -> *)
-(*   ({0;b∅;st}⟦[v:b1|n1|d1|ϕ1]⟧) c2 -> *)
-(*   ({0;b∅;st}⟦-:{v:b1|n1|d1|ϕ1}⤑ τ_x⟧) (vfix (b1 ⤍ b2) (vlam b1 e1)) -> *)
-(*   ({0;b∅;st}⟦ τ_x ^r^ c2 ⟧) (({1 ~t> (vfix (b1 ⤍ b2) (vlam b1 e1))} e1) ^t^ c2). *)
-(* Proof. *)
-(*   intros; subst. *)
-(*   assert (ϕ1 b∅ st c2 /\ [] ⊢t c2 ⋮v b1) as (Hz & HzT). eapply wf_implies_base_phi_sat; eauto. *)
-(*   invclear H2; invclear H1; mydestr. apply H5 in Hz; auto. *)
-(*       apply rR_open_trans_empty' in Hz; auto. *)
-(*       eapply termR_perserve_rR; eauto. refinement_solver. simpl. *)
-(*       apply mk_app_reduce_to_open_fix; auto. refinement_solver. *)
-(* Qed. *)
 
 Lemma wf_implies_base_phi_sat_v: forall m bst st b1 n1 d1 ϕ1 (v2: value),
   (∀ e_wf : tm, ({m;bst;st}⟦[v:b1|n1|d1|ϕ1]⟧) e_wf → ∃ v_wf : value, e_wf ↪* v_wf) ->
@@ -436,8 +200,6 @@ Proof.
   intros. assert (exists c2: constant, v2 = c2) by eauto. mydestr; subst.
   eapply wf_implies_base_phi_sat in H0; eauto.
 Qed.
-
-Check wf_implies_ctxrR_tlete_ubase.
 
 Lemma wf_implies_ctxrR_tlete_ubase_better_drop
      : ∀ (Γ : list (atom * rty)) (st : state) (x : atom) (b : base_ty)
@@ -538,85 +300,6 @@ Proof.
     simpl in H1. termR_solver.
 Qed.
 
-Lemma termR_tletapp_fix: forall Γ e1 (v2: value) e b x1 T,
-    Γ ⊢t v2 ⋮v b -> Γ ⊢t vfix (b ⤍ x1) (vlam b e1) ⋮v b ⤍ x1 ->
-    (exists (L: aset), ∀ y : atom, y ∉ L → (Γ ++ [(y, x1)]) ⊢t e ^t^ y ⋮t T) ->
-  (tlete (({1 ~t> vfix (b ⤍ x1) (vlam b e1)} e1) ^t^ v2) e) <-<{ Γ; T} (tletapp (vfix (b ⤍ x1) (vlam b e1)) v2 e).
-Proof.
-  intros. constructor; auto.
-  - mydestr. econstructor; eauto. apply vfix_implies_open_tyable in H0.
-    simpl in H0. apply vlam_implies_open_tyable with (v2:=v2) in H0; auto.
-  - mydestr. auto_pose_fv x'. eapply tletapp_typable with (x:=x'); eauto; fast_set_solver.
-  - unfold termRraw. intros Γv; intros. reduction_simpl1.
-    rewrite letapp_step_spec. repeat split; auto.
-    + assert (lc (value_msubst Γv (vfix (b ⤍ x1) (vlam b e1)))).
-      eapply instantiation_implies_value_msubst_lc; eauto. basic_typing_solver.
-      msubst_simpl; auto.
-    + reduction_solver1.
-    + apply multi_step_regular in H3; mydestr. lc_solver.
-    + setoid_rewrite tm_open_then_msubst_k in H3; eauto.
-      setoid_rewrite tm_open_then_msubst_k in H3; eauto.
-      right. do 2 eexists; split; eauto.
-      rewrite letapp_step_spec. repeat split; auto.
-      { assert (body (vlam b e1)). basic_typing_solver.
-        assert (body (tm_msubst Γv (vlam b e1))). eapply msubst_preserves_body_tm; eauto.
-        msubst_simpl.
-        eapply open_lc_tm with (u:= vfix (b ⤍ x1) (vlam b (tm_msubst Γv e1))) in H5.
-        msubst_simpl; auto.
-        assert (lc (value_msubst Γv (vfix (b ⤍ x1) (vlam b e1)))).
-      eapply instantiation_implies_value_msubst_lc; eauto. basic_typing_solver.
-      msubst_simpl; auto.
-      }
-      reduction_solver1.
-      apply multi_step_regular in H3; mydestr. lc_solver.
-      left. do 2 eexists; split; eauto. msubst_simpl; auto.
-Qed.
-
-
-Lemma termR_tletapp_lam: forall Γ e1 (v2: value) e Tx Ty T,
-    Γ ⊢t v2 ⋮v Tx -> Γ ⊢t (vlam Tx e1) ⋮v Tx ⤍ Ty ->
-    (exists (L: aset), ∀ y : atom, y ∉ L → (Γ ++ [(y, Ty)]) ⊢t e ^t^ y ⋮t T) ->
-    (tlete (e1 ^t^ v2) e) <-<{Γ; T} (tletapp (vlam Tx e1) v2 e).
-Proof.
-  intros. constructor; auto.
-  - mydestr. econstructor; eauto. invclear H0.
-    auto_pose_fv x'.
-    assert ((Γ ++ [(x', Tx)]) ⊢t e1 ^t^ x' ⋮t Ty). apply H4; fast_set_solver.
-    apply basic_typing_subst_tm_pre with (u:=v2) in H2; auto. lc_simpl4.
-  - mydestr. auto_pose_fv x'. eapply tletapp_typable with (x:=x'); eauto; fast_set_solver.
-  - unfold termRraw. intros Γv; intros. reduction_simpl1.
-    rewrite letapp_step_spec. repeat split; auto.
-    + assert (lc (value_msubst Γv (vlam Tx e1))).
-      eapply instantiation_implies_value_msubst_lc; eauto. basic_typing_solver.
-      msubst_simpl; auto.
-    + reduction_solver1.
-    + apply multi_step_regular in H3; mydestr. lc_solver.
-    + left. do 2 eexists; split; eauto.
-      setoid_rewrite tm_open_then_msubst_k in H3; eauto.
-Qed.
-
-Lemma termR_tletapp_lam_y: forall Γ e1 y (v2: value) e Tx Ty T,
-    Γ ⊢t v2 ⋮v Tx -> Γ ⊢t (vlam Tx e1) ⋮v Tx ⤍ Ty -> y # e ->
-    (Γ ++ [(y, Ty)]) ⊢t e ^t^ y ⋮t T ->
-    (tlete (e1 ^t^ v2) e) <-<{Γ; T} (tletapp (vlam Tx e1) v2 e).
-Proof.
-  intros. constructor; auto.
-  - econstructor; eauto. instantiate (1:=Ty). basic_typing_solver.
-    auto_exists_L_intros.
-    apply basic_has_type_renaming with (x0:=x) in H2; try listctx_set_solver.
-    lc_simpl4. basic_typing_solver.
-  - eapply tletapp_typable with (x:=y); eauto; fast_set_solver.
-  - unfold termRraw. intros Γv; intros. reduction_simpl1.
-    rewrite letapp_step_spec. repeat split; auto.
-    + assert (lc (value_msubst Γv (vlam Tx e1))).
-      eapply instantiation_implies_value_msubst_lc; eauto. basic_typing_solver.
-      msubst_simpl; auto.
-    + reduction_solver1.
-    + apply multi_step_regular in H4; mydestr. lc_solver.
-    + left. do 2 eexists; split; eauto.
-      setoid_rewrite tm_open_then_msubst_k in H4; eauto.
-Qed.
-
 Lemma letapp_aux_typable: forall st τ x τ_x e y,
     x <> y -> x ∉ stale e ->
     (⅋{st}⟦τ⟧{ [(x, τ_x)] } (e ^t^ x)) -> ([(x, ⌊ τ_x ⌋)] ++ [(y, ⌊ τ_x ⌋)]) ⊢t e ^t^ y ⋮t ⌊τ⌋.
@@ -629,87 +312,81 @@ Proof.
   apply basic_typing_weaken_tm_post; auto; listctx_set_solver.
 Qed.
 
-Definition tm_to_value (Tx: ty) (e:tm): value := vlam Tx (mk_app e (vbvar 1)).
+(* Definition tm_to_value (Tx: ty) (e:tm): value := vlam Tx (mk_app e (vbvar 1)). *)
 
-Lemma tm_to_value_typable: forall Γ e Tx T,
-    Γ ⊢t e ⋮t Tx ⤍ T -> Γ ⊢t (tm_to_value Tx e) ⋮v Tx ⤍ T.
-Proof.
-  unfold tm_to_value. intros.
-  auto_exists_L. intros. unfold mk_app.
-  apply mk_app_typable with (T1:=Tx); fold _open_tm.
-  - lc_simpl. basic_typing_solver.
-  - dec_solver1. basic_typing_vfavr_solver.
-Qed.
+(* Lemma tm_to_value_typable: forall Γ e Tx T, *)
+(*     Γ ⊢t e ⋮t Tx ⤍ T -> Γ ⊢t (tm_to_value Tx e) ⋮v Tx ⤍ T. *)
+(* Proof. *)
+(*   unfold tm_to_value. intros. *)
+(*   auto_exists_L. intros. unfold mk_app. *)
+(*   apply mk_app_typable with (T1:=Tx); fold _open_tm. *)
+(*   - lc_simpl. basic_typing_solver. *)
+(*   - dec_solver1. basic_typing_vfavr_solver. *)
+(* Qed. *)
 
-Global Hint Resolve tm_to_value_typable: core.
+(* Global Hint Resolve tm_to_value_typable: core. *)
 
-Lemma mk_app_open: forall e v,
-    lc e -> (mk_app e (vbvar 1) ^t^ v) = mk_app e v.
-Proof.
-  intros. simpl. unfold mk_app. lc_simpl.
-Qed.
+(* Lemma termR_tm_to_value: forall Γ e (v: value) Tx T, *)
+(*     Γ ⊢t e ⋮t Tx ⤍ T -> Γ ⊢t v ⋮v Tx -> *)
+(*     (mk_app e v) <-<{Γ; T} (tletapp (tm_to_value Tx e) v (vbvar 0)). *)
+(* Proof. *)
+(*   intros. *)
+(*   assert (Γ ⊢t tletapp (tm_to_value Tx e) v (vbvar 0) ⋮t T) as HT. *)
+(*   { auto_pose_fv x. eapply tletapp_typable with (x:=x); eauto. fast_set_solver. *)
+(*     simpl. basic_typing_vfavr_solver. } *)
+(*   constructor; auto. *)
+(*   - eapply mk_app_typable; eauto. *)
+(*   - unfold termRraw. intros Γv; intros. *)
+(*     unfold tm_to_value. reduction_simpl1. *)
+(*     rewrite letapp_step_spec; repeat split; auto. *)
+(*     { assert (lc (tm_to_value Tx e)). basic_typing_solver. *)
+(*       eapply instantiation_implies_value_msubst_lc in H3; eauto. *)
+(*       unfold tm_to_value in H3. msubst_simpl; auto. } *)
+(*     reduction_solver1. *)
+(*     left. do 2 eexists; split; eauto. *)
+(*     setoid_rewrite <- tm_open_then_msubst_k; eauto. *)
+(*     rewrite mk_app_open; basic_typing_solver. *)
+(*     rewrite lete_step_spec. split; auto. exists v0. split; auto. simpl. *)
+(*     apply multistep_refl. op_solver1. *)
+(* Qed. *)
 
-Lemma termR_tm_to_value: forall Γ e (v: value) Tx T,
-    Γ ⊢t e ⋮t Tx ⤍ T -> Γ ⊢t v ⋮v Tx ->
-    (mk_app e v) <-<{Γ; T} (tletapp (tm_to_value Tx e) v (vbvar 0)).
-Proof.
-  intros.
-  assert (Γ ⊢t tletapp (tm_to_value Tx e) v (vbvar 0) ⋮t T) as HT.
-  { auto_pose_fv x. eapply tletapp_typable with (x:=x); eauto. fast_set_solver.
-    simpl. basic_typing_vfavr_solver. }
-  constructor; auto.
-  - eapply mk_app_typable; eauto.
-  - unfold termRraw. intros Γv; intros.
-    unfold tm_to_value. reduction_simpl1.
-    rewrite letapp_step_spec; repeat split; auto.
-    { assert (lc (tm_to_value Tx e)). basic_typing_solver.
-      eapply instantiation_implies_value_msubst_lc in H3; eauto.
-      unfold tm_to_value in H3. msubst_simpl; auto. }
-    reduction_solver1.
-    left. do 2 eexists; split; eauto.
-    setoid_rewrite <- tm_open_then_msubst_k; eauto.
-    rewrite mk_app_open; basic_typing_solver.
-    rewrite lete_step_spec. split; auto. exists v0. split; auto. simpl.
-    apply multistep_refl. op_solver1.
-Qed.
+(* Lemma termR_tm_to_value': forall Γ e (v: value) Tx T, *)
+(*     Γ ⊢t e ⋮t Tx ⤍ T -> Γ ⊢t v ⋮v Tx -> *)
+(*     (tletapp (tm_to_value Tx e) v (vbvar 0)) <-<{Γ; T} (mk_app e v). *)
+(* Proof. *)
+(*   intros. *)
+(*   assert (Γ ⊢t tletapp (tm_to_value Tx e) v (vbvar 0) ⋮t T) as HT. *)
+(*   { auto_pose_fv x. eapply tletapp_typable with (x:=x); eauto. fast_set_solver. *)
+(*     simpl. basic_typing_vfavr_solver. } *)
+(*   constructor; auto. *)
+(*   - eapply mk_app_typable; eauto. *)
+(*   - unfold termRraw. intros Γv; intros. *)
+(*     unfold tm_to_value in H2. reduction_simpl1. *)
+(*     rewrite letapp_step_spec in H2; mydestr. destruct H5; mydestr; invclear H5. *)
+(*     setoid_rewrite <- tm_open_then_msubst_k in H6; eauto. *)
+(*     rewrite mk_app_open in H6; basic_typing_solver. *)
+(*     eapply lete_0_reduce_to_self_aux'; eauto. msubst_simpl; auto. *)
+(* Qed. *)
 
-Lemma termR_tm_to_value': forall Γ e (v: value) Tx T,
-    Γ ⊢t e ⋮t Tx ⤍ T -> Γ ⊢t v ⋮v Tx ->
-    (tletapp (tm_to_value Tx e) v (vbvar 0)) <-<{Γ; T} (mk_app e v).
-Proof.
-  intros.
-  assert (Γ ⊢t tletapp (tm_to_value Tx e) v (vbvar 0) ⋮t T) as HT.
-  { auto_pose_fv x. eapply tletapp_typable with (x:=x); eauto. fast_set_solver.
-    simpl. basic_typing_vfavr_solver. }
-  constructor; auto.
-  - eapply mk_app_typable; eauto.
-  - unfold termRraw. intros Γv; intros.
-    unfold tm_to_value in H2. reduction_simpl1.
-    rewrite letapp_step_spec in H2; mydestr. destruct H5; mydestr; invclear H5.
-    setoid_rewrite <- tm_open_then_msubst_k in H6; eauto.
-    rewrite mk_app_open in H6; basic_typing_solver.
-    eapply lete_0_reduce_to_self_aux'; eauto. msubst_simpl; auto.
-Qed.
+(* Lemma termR_tm_to_value_mk_app: forall Γ e (v: value) Tx T, *)
+(*     Γ ⊢t e ⋮t Tx ⤍ T -> Γ ⊢t v ⋮v Tx -> *)
+(*     (mk_app e v) <-<{Γ; T} (mk_app (tm_to_value Tx e) v). *)
+(* Proof. *)
+(*   intros. *)
+(*   apply termR_trans_better with (tletapp (tm_to_value Tx e) v (vbvar 0)). *)
+(*   - eapply termR_tm_to_value; auto. *)
+(*   - eapply mk_app_v_v_reduce_to_letapp'; eauto. *)
+(* Qed. *)
 
-Lemma termR_tm_to_value_mk_app: forall Γ e (v: value) Tx T,
-    Γ ⊢t e ⋮t Tx ⤍ T -> Γ ⊢t v ⋮v Tx ->
-    (mk_app e v) <-<{Γ; T} (mk_app (tm_to_value Tx e) v).
-Proof.
-  intros.
-  apply termR_trans_better with (tletapp (tm_to_value Tx e) v (vbvar 0)).
-  - eapply termR_tm_to_value; auto.
-  - eapply mk_app_v_v_reduce_to_letapp'; eauto.
-Qed.
-
-Lemma termR_tm_to_value_mk_app': forall Γ e (v: value) Tx T,
-    Γ ⊢t e ⋮t Tx ⤍ T -> Γ ⊢t v ⋮v Tx ->
-    (mk_app (tm_to_value Tx e) v) <-<{Γ; T} (mk_app e v).
-Proof.
-  intros.
-  apply termR_trans_better with (tletapp (tm_to_value Tx e) v (vbvar 0)).
-  - eapply mk_app_v_v_reduce_to_letapp; eauto.
-  - eapply termR_tm_to_value'; auto.
-Qed.
+(* Lemma termR_tm_to_value_mk_app': forall Γ e (v: value) Tx T, *)
+(*     Γ ⊢t e ⋮t Tx ⤍ T -> Γ ⊢t v ⋮v Tx -> *)
+(*     (mk_app (tm_to_value Tx e) v) <-<{Γ; T} (mk_app e v). *)
+(* Proof. *)
+(*   intros. *)
+(*   apply termR_trans_better with (tletapp (tm_to_value Tx e) v (vbvar 0)). *)
+(*   - eapply mk_app_v_v_reduce_to_letapp; eauto. *)
+(*   - eapply termR_tm_to_value'; auto. *)
+(* Qed. *)
 
 Definition arg_ty (τ: rty): ty :=
   match τ with
@@ -718,44 +395,35 @@ Definition arg_ty (τ: rty): ty :=
   | _ => ⌊ τ ⌋
   end.
 
-Lemma rR_is_arr_refine: forall m bst st τ_x e,
-    is_arr τ_x ->
-    {m;bst;st}⟦τ_x⟧ e ->
-    {m;bst;st}⟦τ_x⟧ (tm_to_value (arg_ty τ_x) e).
-Proof.
-  intros. destruct τ_x; auto_ty_exfalso.
-  - invclear H0; mydestr.
-    constructor; auto. denotation_simp. constructor; auto.
-    intros. apply H2 in H4; auto.
-    eapply termR_perserve_rR; eauto; refinement_solver.
-    apply termR_tm_to_value_mk_app; auto.
-  - invclear H0; mydestr.
-    constructor; auto. denotation_simp. constructor; auto.
-    intros. auto_under v_x.
-    eapply termR_perserve_rR; eauto; refinement_solver.
-    apply termR_tm_to_value_mk_app; auto. refinement_solver.
-Qed.
+(* Lemma rR_is_arr_refine: forall m bst st τ_x e, *)
+(*     is_arr τ_x -> *)
+(*     {m;bst;st}⟦τ_x⟧ e -> *)
+(*     {m;bst;st}⟦τ_x⟧ (tm_to_value (arg_ty τ_x) e). *)
+(* Proof. *)
+(*   intros. destruct τ_x; auto_ty_exfalso. *)
+(*   - invclear H0; mydestr. *)
+(*     constructor; auto. denotation_simp. constructor; auto. *)
+(*     intros. apply H2 in H4; auto. *)
+(*     eapply termR_perserve_rR; eauto; refinement_solver. *)
+(*     apply termR_tm_to_value_mk_app; auto. *)
+(*   - invclear H0; mydestr. *)
+(*     constructor; auto. denotation_simp. constructor; auto. *)
+(*     eexists (tm_to_value (arg_ty (τ_x1 ⤑ τ_x2)) e). split; auto. admit. *)
+(*     intros. auto_under v_x. *)
+(*     eapply termR_perserve_rR; eauto; refinement_solver. *)
+(*     apply termR_tm_to_value_mk_app; auto. refinement_solver. *)
+(* Qed. *)
 
-Lemma termR_elete_better
-  : ∀ (γ : listctx ty) (Tx T : ty) (e_x e_x' e e' : tm) (x : atom),
-    x ∉ stale e ∪ stale e' ->
-    e_x <-<{ γ; Tx} e_x'
-    → (e ^t^ x) <-<{ γ ++ [(x, Tx)]; T}(e' ^t^ x)
-    → (tlete e_x e) <-<{ γ; T} (tlete e_x' e').
+Lemma rR_arr_halt: forall m bst st τ e,
+    is_arr τ -> {m;bst;st}⟦τ⟧ e -> (exists (v: value), {m;bst;st}⟦τ⟧ v /\ e ↪* v).
 Proof.
-  intros.
-  eapply termR_elete in H1; eauto.
-  rewrite close_open_var_tm in H1; try fast_set_solver.
-  rewrite close_open_var_tm in H1; try fast_set_solver.
-Qed.
-
-Lemma termR_elete_lhs
-  : ∀ (γ : listctx ty) (Tx T : ty) (e_x e_x' e : tm) (x : atom),
-    x ∉ stale e ->
-    e_x <-<{ γ; Tx} e_x' -> (γ ++ [(x, Tx)]) ⊢t (e ^t^ x) ⋮t T
-    → (tlete e_x e) <-<{ γ; T} (tlete e_x' e).
-Proof.
-  intros. eapply termR_elete_better; eauto. fast_set_solver.
+  intros. destruct τ; try auto_ty_exfalso.
+  - simpl in H0; mydestr. exists x; split; auto.
+    constructor; auto. reduction_solver1. split; auto.
+    eexists; split; eauto. reduction_solver1.
+  - simpl in H0; mydestr. exists x; split; auto.
+    constructor; auto. reduction_solver1. split; auto.
+    eexists; split; eauto. reduction_solver1.
 Qed.
 
 Lemma rR_letapp_base': forall τ_x τ st x (v1 v2: value) (e: tm) b n d ϕ,
@@ -766,8 +434,8 @@ Lemma rR_letapp_base': forall τ_x τ st x (v1 v2: value) (e: tm) b n d ϕ,
     {0;b∅;st}⟦-:{v: b | n | d | ϕ}⤑ τ_x⟧ v1 ->
     {0;b∅;st}⟦[v:b|n|d|ϕ]⟧ v2 ->
     (⅋{st}⟦τ⟧{[(x, τ_x ^r^ v2)] }) (e ^t^ x) ->
-    {0;b∅;st}⟦τ⟧ (tletapp v1 v2 e).
-    (* (⅋{st}⟦τ⟧{[(x, τ_x ^r^ v2)] }) (tletapp v1 v2 e). *)
+    (* {0;b∅;st}⟦τ⟧ (tletapp v1 v2 e). *)
+    (⅋{st}⟦τ⟧{[(x, τ_x ^r^ v2)] }) (tletapp v1 v2 e).
 Proof.
   intros.
   assert (exists c2: constant, v2 = c2 /\ ϕ b∅ st c2 /\ [] ⊢t c2 ⋮v b); mydestr; subst.
@@ -777,24 +445,35 @@ Proof.
     + rename x1 into e1.
       assert (({0;b∅;st}⟦τ_x ^r^ x0⟧) (e1 ^t^ x0)) as Hz.
       { eapply rR_letapp_overbase_lam in H4; eauto. }
-      invclear H6; try auto_ty_exfalso5.
-      simpl in H4; mydestr.
-      constructor; auto. admit. admit. admit.
-      apply rR_is_arr_refine in Hz; auto.
-      apply wf_implies_ctxrR_tlete_is_arr_better_empty with (x:=x) (e:=e) (τ:=τ) in Hz; eauto; try fast_set_solver.
+      assert (is_arr (τ_x ^r^ x0)) as Hzz; auto.
+      pose (rR_arr_halt _ _ _ _ _ Hzz Hz). mydestr.
+      apply wf_implies_ctxrR_tlete_is_arr_better_empty with (x:=x) (e:=e) (τ:=τ) in H7; eauto; try fast_set_solver.
       eapply termR_perserve_inv_ctxrR; eauto.
-      { invclear Hz; refinement_solver. }
-      simpl. inv_rd_simpl1.
-      apply termR_trans_better with ((tlete (e1 ^t^ x0) e)).
-      { apply termR_elete_lhs with (x:=x) (Tx := ⌊τ_x⌋). fast_set_solver.
-
-        eapply termR_elete. }
-      admit.
-      apply termR_tletapp_lam with (Ty := ⌊τ_x ⌋ ); eauto.
+      { invclear H7; refinement_solver. }
+      apply termR_trans_better with (tlete (e1 ^t^ x0) e).
+      simpl. apply termR_weakening. listctx_set_solver.
+      eapply termR_elete_lhs with (x:=x); eauto; try inv_rd_simpl1.
+      apply termR_value_tm; auto; refinement_solver.
+      simpl. apply termR_tletapp_lam with (Ty := ⌊ τ_x ⌋); auto; inv_rd_simpl1.
       basic_typing_solver. refinement_solver. basic_typing_solver.
       auto_exists_L. intros.
-      eapply letapp_aux_typable in H6; inv_rd_simpl1; eauto.
-    + admit.
+      eapply letapp_aux_typable in H6; eauto; inv_rd_simpl1.
+    + rename x1 into e1.
+      assert (({0;b∅;st}⟦τ_x ^r^ x0⟧) (({1 ~t> x0} e1) ^t^ (vfix (b ⤍ ⌊τ_x⌋) (vlam b e1)))) as Hz.
+      { eapply rR_letapp_overbase_fix in H4; eauto. }
+      assert (is_arr (τ_x ^r^ x0)) as Hzz; auto.
+      pose (rR_arr_halt _ _ _ _ _ Hzz Hz). mydestr.
+      apply wf_implies_ctxrR_tlete_is_arr_better_empty with (x:=x) (e:=e) (τ:=τ) in H7; eauto; try fast_set_solver.
+      eapply termR_perserve_inv_ctxrR; eauto.
+      { invclear H7; refinement_solver. }
+      apply termR_trans_better with (tlete (({1 ~t> x0} e1) ^t^ (vfix (b ⤍ ⌊τ_x⌋) (vlam b e1))) e).
+      apply termR_weakening. listctx_set_solver.
+      eapply termR_elete_lhs with (x:=x); eauto; try inv_rd_simpl1.
+      apply termR_value_tm; auto; refinement_solver.
+      simpl. apply termR_tletapp_fix; auto.
+      basic_typing_solver. refinement_solver. basic_typing_solver.
+      auto_exists_L. intros.
+      eapply letapp_aux_typable in H6; eauto; inv_rd_simpl1.
   - destruct τ_x; try auto_ty_exfalso. invclear H1.
     destruct (rR_arrow_value_lam_exists_oarr _ _ _ _ _ _ _ _ _ H4); mydestr; subst.
     + rename x5 into e1.
@@ -808,7 +487,7 @@ Proof.
       auto_exists_L. intros.
       eapply letapp_aux_typable in H6; eauto; fast_set_solver.
     + rename x5 into e1.
-      assert (({0;b∅;st}⟦[v:x1|x2|x3|x4] ^r^ x0⟧) (({1 ~t> vfix (b ⤍ x1) (vlam b e1)} e1) ^t^ x0)) as Hz.
+      assert (({0;b∅;st}⟦[v:x1|x2|x3|x4] ^r^ x0⟧) (({1 ~t> x0} e1) ^t^ (vfix (b ⤍ x1) (vlam b e1)))) as Hz.
       { eapply rR_letapp_overbase_fix in H4; eauto. }
       apply wf_implies_ctxrR_tlete_ubase_better_empty with (x:=x) (e:=e) (τ:=τ) in Hz; eauto; try fast_set_solver.
       eapply termR_perserve_inv_ctxrR; eauto.
@@ -817,160 +496,4 @@ Proof.
       basic_typing_solver. refinement_solver. basic_typing_solver.
       auto_exists_L. intros.
       eapply letapp_aux_typable in H6; eauto; fast_set_solver.
-Admitted.
-
-
-
-
-Lemma rR_letapp_base: forall τ st τ_x (v1 v2 v_x: value) (e: tm) b n d ϕ,
-  not_overbasety τ -> not_overbasety τ_x ->
-  (∀ e_wf : tm, ({0;b∅;st}⟦[v:b|n|d|ϕ]⟧) e_wf → ∃ v_wf : value, e_wf ↪* v_wf) ->
-  (∀ e_wf : tm, ({0;b∅;st}⟦τ_x ^r^ v2⟧) e_wf → ∃ v_wf : value, e_wf ↪* v_wf) ->
-  ({0;b∅;st}⟦[v:b|n|d|ϕ]⟧) v2 ->
-  ({0;b∅;st}⟦-:{v: b | n | d | ϕ}⤑ τ_x⟧) v1 ->
-  ({0;b∅;st}⟦τ_x ^r^ v2⟧) v_x ->
-  ({0;b∅;st}⟦τ⟧) (e ^t^ v_x) ->
-  ({0;b∅;st}⟦τ⟧) (tletapp v1 v2 e).
-Proof.
-  intros. apply termR_perserve_rR with (e ^t^ v_x); auto; refinement_solver.
-  constructor; refinement_solver.
-  - inv_rd_simpl1. admit.
-  - unfold termRraw. intros. instantiation_simp.
-    simpl in H4. mydestr.
-    assert (exists (c2: constant), v2 = c2); mydestr; subst. { admit. }
-    assert (ϕ b∅ st x). admit.
-    apply H9 in H10; refinement_solver.
-    apply rR_open_trans_empty' in H10.
-Admitted.
-
-Lemma rR_letapp_base_lam: forall τ st τ_x x e1 (v2: value) (e: tm) b n d ϕ,
-    x ∉ fv_tm e ∪ rty_fv τ ->
-    not_overbasety τ -> not_overbasety τ_x ->
-    (∀ e_wf : tm, ({0;b∅;st}⟦[v:b|n|d|ϕ]⟧) e_wf → ∃ v_wf : value, e_wf ↪* v_wf) ->
-    (∀ e_wf : tm, ({0;b∅;st}⟦τ_x ^r^ v2⟧) e_wf → ∃ v_wf : value, e_wf ↪* v_wf) ->
-    {0;b∅;st}⟦-:{v: b | n | d | ϕ}⤑ τ_x⟧ (vlam b e1) ->
-    {0;b∅;st}⟦[v:b|n|d|ϕ]⟧ v2 ->
-    {0;b∅;st}⟦τ_x ^r^ v2⟧ (e1 ^t^ v2).
-Admitted.
-
-Lemma rR_letapp_base_fun: forall τ st τ_x x (v1 v2: value) (e: tm) b n d ϕ,
-    x ∉ fv_tm e ∪ rty_fv τ ->
-    not_overbasety τ -> not_overbasety τ_x ->
-    (∀ e_wf : tm, ({0;b∅;st}⟦[v:b|n|d|ϕ]⟧) e_wf → ∃ v_wf : value, e_wf ↪* v_wf) ->
-    (∀ e_wf : tm, ({0;b∅;st}⟦τ_x ^r^ v2⟧) e_wf → ∃ v_wf : value, e_wf ↪* v_wf) ->
-    {0;b∅;st}⟦-:{v: b | n | d | ϕ}⤑ τ_x⟧ v1 ->
-    {0;b∅;st}⟦[v:b|n|d|ϕ]⟧ v2 ->
-    (exists v_x: value, {0;b∅;st}⟦τ_x ^r^ v2⟧ v_x /\ v_x <-<{ []; b ⤍ ⌊ τ_x ⌋} (mk_app v1 v2)).
-Admitted.
-
-Lemma rR_letapp_base_app_x_arr: forall τ st τ_x x (v1 v2: value) (v_x: value) (e: tm),
-    x ∉ fv_tm e ∪ rty_fv τ ->
-    not_overbasety τ -> is_arr τ_x ->
-    {0;b∅;st}⟦τ_x⟧ v_x ->
-    v_x <-<{ []; b ⤍ ⌊ τ_x ⌋} (mk_app v1 v2) ->
-    (⅋{st}⟦τ⟧{[(x, τ_x)] }) (e ^t^ x) ->
-    {0;b∅;st}⟦τ⟧ (tletapp v1 v2 e).
-Proof.
-
-Lemma rR_letapp_base': forall τ st τ_x x (v1 v2: value) (e: tm) b n d ϕ,
-    x ∉ fv_tm e ∪ rty_fv τ ->
-    not_overbasety τ -> not_overbasety τ_x ->
-    (∀ e_wf : tm, ({0;b∅;st}⟦[v:b|n|d|ϕ]⟧) e_wf → ∃ v_wf : value, e_wf ↪* v_wf) ->
-    (∀ e_wf : tm, ({0;b∅;st}⟦τ_x ^r^ v2⟧) e_wf → ∃ v_wf : value, e_wf ↪* v_wf) ->
-    {0;b∅;st}⟦-:{v: b | n | d | ϕ}⤑ τ_x⟧ v1 ->
-    {0;b∅;st}⟦[v:b|n|d|ϕ]⟧ v2 ->
-    (⅋{st}⟦τ⟧{[(x, τ_x ^r^ v2)] }) (e ^t^ x) ->
-    (⅋{st}⟦τ⟧{[(x, τ_x ^r^ v2)] }) (tletapp v1 v2 e).
-Proof.
-  intros. eapply rR_letapp_base_fun in H4; eauto.
-  mydestr. invclear H6. admit. constructor; auto. admit.
-  exists x0. split; auto. admit. intros.
-
-Lemma rR_letapp_base': forall τ st τ_x x e1 (v2: value) (e: tm) b n d ϕ,
-    x ∉ fv_tm e ∪ rty_fv τ ->
-    not_overbasety τ -> not_overbasety τ_x ->
-    (∀ e_wf : tm, ({0;b∅;st}⟦[v:b|n|d|ϕ]⟧) e_wf → ∃ v_wf : value, e_wf ↪* v_wf) ->
-    (∀ e_wf : tm, ({0;b∅;st}⟦τ_x ^r^ v2⟧) e_wf → ∃ v_wf : value, e_wf ↪* v_wf) ->
-    {0;b∅;st}⟦-:{v: b | n | d | ϕ}⤑ τ_x⟧ (vlam b e1) ->
-    {0;b∅;st}⟦[v:b|n|d|ϕ]⟧ v2 ->
-    (⅋{st}⟦τ⟧{[(x, τ_x ^r^ v2)] }) (e ^t^ x) ->
-    (⅋{st}⟦τ⟧{[(x, τ_x ^r^ v2)] }) (tletapp (vlam b e1) v2 e).
-Proof.
-  intros. eapply rR_letapp_base_fun in H4; eauto.
-  assert ((⅋{st}⟦τ⟧{[] ++ [(x, τ_x ^r^ v2)] }) (tlete (e1 ^t^ v2) (x \t\ (e ^t^ x)))).
-  Check wf_implies_ctxrR_tlete_is_arr.
-  apply wf_implies_ctxrR_tlete_is_arr.
-
-  invclear H6; try auto_ty_exfalso5. admit. (e1^v2)
-
-  assert
-    ((∃ e : tm, v1 = vlam b e) ∨ (∃ e : tm, v1 = vfix (b ⤍ ⌊ τ_x ⌋) (vlam b e))).
-  eapply rR_arrow_value_lam_exists_oarr; eauto. destruct H7; mydestr; subst.
-
-
-
-  apply termR_perserve_rR with (e ^t^ v_x); auto; refinement_solver.
-  constructor; refinement_solver.
-  - inv_rd_simpl1. admit.
-  - unfold termRraw. intros. instantiation_simp.
-    simpl in H4. mydestr.
-    assert (exists (c2: constant), v2 = c2); mydestr; subst. { admit. }
-    assert (ϕ bst st x). admit.
-    apply H9 in H10; refinement_solver.
-Admitted.
-
-Lemma inv_rRctx_letapp_oarr: forall Γ st (τ: rty) b n d ϕ x τ_x (v1 v2: value) e,
-    x ∉ fv_tm e ∪ rty_fv τ -> not_overbasety τ -> not_overbasety τ_x ->
-    closed_rty 0 (ctxdom ⦑Γ⦒ ∪ dom aset st) τ ->
-    wf_ctxrR st (Γ ++ [(x, [v:b|n|d|ϕ])]) ->
-    wf_ctxrR st (Γ ++ [(x, τ_x ^r^ v2)]) ->
-    (⅋{st}⟦-:{v: b | n | d | ϕ}⤑ τ_x⟧{Γ}) v1 ->
-    (⅋{st}⟦[v:b|n|d|ϕ]⟧{Γ}) v2 ->
-    (⅋{st}⟦τ⟧{Γ ++ [(x, τ_x ^r^ v2)] }) (e ^t^ x) ->
-    ⅋{st}⟦τ⟧{Γ ++ [(x, τ_x ^r^ v2)] } (tletapp v1 v2 e).
-Proof.
-    induction Γ; intros.
-    - mydestr. inv_rd_simpl1.
-      invclear H5. destruct (decide (is_arr τ_x)).
-      + constructor; auto. wf_regular_solver. denotation_simp.
-        inv_rd_simpl2. inv_rd_simpl1. inv_rd_simpl3. inv_rd_simpl1.
-        apply basic_typing_weaken_tm_empty; eauto. listctx_set_solver.
-        eapply tletapp_typable with (x:=x) (Γ:=[]); eauto; basic_typing_solver.
-        intros. constructor; auto. RD_simp2; try auto_ty_exfalso5. clear H25.
-    rewrite subst_fresh_tm. lc_simpl4.
-    assert (({0;b∅;st}⟦τ_x ^r^ v2⟧) (v1 ) )
-
-    specialize (H19 _ H8).  RD_simp2. lc_simpl4. simpl.
-        rewrite subst_fresh_value. rewrite subst_fresh_value.
-        rewrite subst_fresh_tm.
-        admit. fast_set_solver.
-        
-      rewrite open_subst_same_tm in H6; auto. admit. fast_set_solver. try clear Htmp
-
-        admit.
-      + auto_ty_exfalso. RD_simp2. mydestr. constructor; auto.
-        admit. exists x5. split; auto. intros. auto_under v_x. RD_simp2. dsimp1. admit.
-    - RD_simp2.
-      + constructor; auto. admit. intros. auto_under c_x.
-        assert ((⅋{<[a:=c_x]> st}⟦τ⟧{Γ ++ [(x, τ_x ^r^ ({a := c_x }v v2))] })
-                  (tletapp ({a := c_x }v v1) ({a := c_x }v v2) ({a := c_x }t e))).
-        eapply IHΓ; eauto. admit. admit. admit. admit. admit.
-      + constructor; auto. admit.
-        mydestr. auto_meet_exists Hmeet. auto_meet_reduce. auto_under v_x.
-        admit.
-      + constructor; auto. denotation_simp. admit.
-        intros. auto_under v_x.
-
-
-    + denotation_simp. assert ([] ⊢t tletbiop op v1 v2 e ⋮t ⌊τ⌋). eapply tletbiop_typable; refinement_solver.
-      basic_typing_solver.
-    + assert ((exists (m1: nat), v1 = m1)) by (eapply fst_ty_of_op_implies_nat; eauto). mydestr; subst. rename x2 into v1.
-      assert ((exists (m2: nat), v2 = m2)) by (eapply snd_ty_of_op_implies_nat; eauto). mydestr; subst. rename x2 into v2.
-      exists (eval_op_under_bound_tm op v1 v2). split. apply rR_eval_op_under_bound_tm.
-      intros. assert (x1 ↪* v_x) as Hz by (eapply rR_eval_op_under_bound_tm_min; eauto).
-      auto_under v_x. RD_simp2. simpl.
-      rewrite subst_fresh_tm; auto. rewrite open_subst_same_tm in H10; auto.
-      eapply termR_perserve_rR; refinement_solver.
-      eapply letapp_eval_op_under_bound_tm_termR; eauto; refinement_solver.
-
-
+Qed.
