new_proof/RDInv5.v
@@ -1,0 +1,543 @@
+From stdpp Require Import mapset.
+From stdpp Require Import natmap.
+From stdpp Require Import fin_map_dom.
+From CT Require Import CoreLangProp.
+From CT Require Import OperationalSemanticsProp.
+From CT Require Import BasicTypingProp.
+From CT Require Import SyntaxSugar.
+From CT Require Import Refinement.
+From CT Require Import RefinementTac.
+From CT Require Import RefinementDenotation.
+From CT Require Import RefinementDenotationTac.
+From CT Require Import RefinementDenotationProp.
+From CT Require Import RDInv.
+From CT Require Import RDInv2.
+From CT Require Import RDInv3.
+From CT Require Import RDInv4.
+From CT Require Import TermOrdering.
+From Coq Require Import Logic.ClassicalFacts.
+From Coq Require Import Classical.
+
+Import Atom.
+Import CoreLang.
+Import CoreLangProp.
+Import Tactics.
+Import NamelessTactics.
+Import ListCtx.
+Import OperationalSemantics.
+Import OperationalSemanticsProp.
+Import BasicTyping.
+Import SyntaxSugar.
+Import Refinement.
+Import RefinementTac.
+Import RefinementDenotation.
+Import RefinementDenotationTac.
+Import RefinementDenotationProp.
+Import NamelessTactics.
+Import TermOrdering.
+Import RDInv.
+Import RDInv2.
+Import RDInv3.
+Import RDInv4.
+
+Global Hint Resolve mk_eq_constant_is_not_overbasety: core.
+Global Hint Resolve mk_eq_var_is_not_overbasety: core.
+Global Hint Resolve is_arr_implies_not_overbasety: core.
+Global Hint Constructors ok_dctx: core.
+Global Hint Resolve rR_implies_no_free: core.
+Global Hint Resolve ctxrR_tlete_drop_halt_lhs: core.
+Global Hint Resolve rR_implies_reduction_no_free: core.
+Global Hint Resolve is_arr_implies_not_overbasety: core.
+Global Hint Resolve under_not_overbasety: core.
+
+Lemma rR_mk_eq_constant: forall c, ({0;b∅;∅}⟦mk_eq_constant c⟧) c.
+Proof.
+  unfold mk_eq_constant. intros. simpl.
+  constructor; auto. constructor; auto.
+  - repeat (constructor; auto). fast_set_solver.
+  - intros; subst; auto.
+Qed.
+
+Global Hint Resolve rR_mk_eq_constant: core.
+
+Lemma rR_mk_under_bot_terr: forall b, ({0;b∅;∅}⟦mk_under_bot b⟧) terr.
+Proof.
+  unfold mk_under_bot. intros. simpl.
+  constructor; auto. constructor; auto.
+  - repeat (constructor; auto). fast_set_solver.
+  - intros; subst; auto. invclear H0.
+Qed.
+
+Global Hint Resolve rR_mk_under_bot_terr: core.
+
+Lemma rR_mk_eq_constant_bool: forall st (b: bool) (v: value),
+  ({0;b∅;st}⟦mk_eq_constant b⟧) v -> v = b.
+Proof.
+  intros. simpl in H; mydestr.
+  assert ([] ⊢t b ⋮v TBool). constructor; auto.
+  apply H1 in H2; auto. reduction_simpl1. auto.
+Qed.
+
+Lemma termR_tmatchb_true: forall Γ T e1 e2,
+  Γ ⊢t e1 ⋮t T -> Γ ⊢t e2 ⋮t T ->
+  e1 <-<{ Γ; T} (tmatchb true e1 e2).
+Proof.
+  intros. constructor; auto.
+  - repeat constructor; auto. basic_typing_solver.
+  - unfold termRraw. intros Γv; intros. assert (closed_value true) by auto.
+    reduction_simpl1. rewrite value_msubst_closed; auto.
+    eapply multistep_step; eauto. constructor; auto; reduction_solver1.
+Qed.
+
+Lemma termR_tmatchb_false: forall Γ T e1 e2,
+  Γ ⊢t e1 ⋮t T -> Γ ⊢t e2 ⋮t T ->
+  e2 <-<{ Γ; T} (tmatchb false e1 e2).
+Proof.
+  intros. constructor; auto.
+  - repeat constructor; auto. basic_typing_solver.
+  - unfold termRraw. intros Γv; intros. assert (closed_value false) by auto.
+    reduction_simpl1. rewrite value_msubst_closed; auto.
+    eapply multistep_step; eauto. constructor; auto; reduction_solver1.
+Qed.
+
+Lemma inv_rRctx_matchb_true: forall Γ st (τ: rty) (v: value) e1 e2,
+    not_overbasety τ ->
+    closed_rty 0 (ctxdom ⦑Γ⦒ ∪ dom aset st) τ ->
+    wf_ctxrR st Γ ->
+    (⅋{st}⟦mk_eq_constant true⟧{Γ}) v ->
+    (⅋{st}⟦τ⟧{Γ}) e1 ->
+    ⌊ Γ ⌋* ⊢t e2 ⋮t ⌊ τ ⌋ ->
+    (⅋{st}⟦τ⟧{Γ}) (tmatchb v e1 e2).
+Proof.
+  induction Γ; intros.
+  { RD_simp2. apply rR_mk_eq_constant_bool in H3; subst. eapply termR_perserve_rR; eauto.
+    refinement_solver. apply termR_tmatchb_true; auto. refinement_solver. }
+  mydestr.
+  assert (a ∉ dom aset st ∪ ctxdom Γ) as Ha. { RD_simp2; refinement_solver. }
+  assert (((a, ⌊ r ⌋) :: ⌊Γ⌋*) ⊢t (tmatchb v e1 e2) ⋮t ⌊τ⌋) as HT by inv_rd_simpl1.
+  RD_simp2; constructor; auto.
+ - intros. auto_under c_x.
+            eapply IHΓ; eauto; fold value_subst; fold tm_subst.
+            + refinement_solver.
+            + eapply basic_typing_subst_tm_post in H4; eauto.
+              refinement_solver.
+          - mydestr. auto_meet_exists HE.
+            auto_meet_reduce. dsimp1. rename x2 into c_x. auto_under x0.
+            eapply IHΓ; eauto; fold value_subst; fold tm_subst.
+            + refinement_solver.
+            + eapply basic_typing_subst_tm_post; eauto.
+          - intros. auto_under v_x.
+            apply IHΓ; eauto; fold value_subst; fold tm_subst.
+            eapply basic_typing_subst_tm_post in H4; eauto. refinement_solver.
+Qed.
+
+Lemma inv_rRctx_matchb_false: forall Γ st (τ: rty) (v: value) e1 e2,
+    not_overbasety τ ->
+    closed_rty 0 (ctxdom ⦑Γ⦒ ∪ dom aset st) τ ->
+    wf_ctxrR st Γ ->
+    (⅋{st}⟦mk_eq_constant false⟧{Γ}) v ->
+    (⅋{st}⟦τ⟧{Γ}) e2 ->
+    ⌊ Γ ⌋* ⊢t e1 ⋮t ⌊ τ ⌋ ->
+    (⅋{st}⟦τ⟧{Γ}) (tmatchb v e1 e2).
+Proof.
+  induction Γ; intros.
+  { RD_simp2. apply rR_mk_eq_constant_bool in H3; subst. eapply termR_perserve_rR; eauto.
+    refinement_solver. apply termR_tmatchb_false; auto. refinement_solver. }
+  mydestr.
+  assert (a ∉ dom aset st ∪ ctxdom Γ) as Ha. { RD_simp2; refinement_solver. }
+  assert (((a, ⌊ r ⌋) :: ⌊Γ⌋*) ⊢t (tmatchb v e1 e2) ⋮t ⌊τ⌋) as HT by inv_rd_simpl1.
+  RD_simp2; constructor; auto.
+ - intros. auto_under c_x.
+            eapply IHΓ; eauto; fold value_subst; fold tm_subst.
+            + refinement_solver.
+            + eapply basic_typing_subst_tm_post in H4; eauto.
+              refinement_solver.
+          - mydestr. auto_meet_exists HE.
+            auto_meet_reduce. dsimp1. rename x2 into c_x. auto_under x0.
+            eapply IHΓ; eauto; fold value_subst; fold tm_subst.
+            + refinement_solver.
+            + eapply basic_typing_subst_tm_post; eauto.
+          - intros. auto_under v_x.
+            apply IHΓ; eauto; fold value_subst; fold tm_subst.
+            eapply basic_typing_subst_tm_post in H4; eauto. refinement_solver.
+Qed.
+
+Lemma inv_rRctx_letapp_oarr: forall Γ st (τ: rty) b n d ϕ x τ_x (v1 v2: value) e,
+    x ∉ fv_tm e ∪ rty_fv τ -> not_overbasety τ -> not_overbasety τ_x ->
+    closed_rty 0 (ctxdom ⦑Γ⦒ ∪ dom aset st) τ ->
+    wf_ctxrR st (Γ ++ [(x, [v:b|n|d|ϕ])]) ->
+    wf_ctxrR st (Γ ++ [(x, τ_x ^r^ v2)]) ->
+    (⅋{st}⟦-:{v: b | n | d | ϕ}⤑ τ_x⟧{Γ}) v1 ->
+    (⅋{st}⟦[v:b|n|d|ϕ]⟧{Γ}) v2 ->
+    (⅋{st}⟦τ⟧{Γ ++ [(x, τ_x ^r^ v2)] }) (e ^t^ x) ->
+    ⅋{st}⟦τ⟧{Γ ++ [(x, τ_x ^r^ v2)] } (tletapp v1 v2 e).
+Proof.
+    induction Γ; intros.
+    invclear H5. invclear H6. invclear H3; try auto_ty_exfalso.
+    eapply rR_letapp_base'; eauto.
+    assert ((exists (n: constant), v2 = n) \/ (exists (y: atom), v2 = y)) as Hv2.
+    { invclear H6; eapply has_basety_implies_constant_or_var; eauto;
+      basic_typing_solver. }
+    mydestr.
+    assert (a ∉ dom aset st ∪ ctxdom Γ ∪ {[x]}) as Ha.
+    { RD_simp2; refinement_solver. }
+    RD_simp2; constructor; auto.
+    - denotation_simp. apply cons_basic_typing_drop_last_tm.
+      refinement_solver.
+      eapply tletapp_typable with (x:=x); eauto.
+      fast_set_solver. inv_rd_simpl1.
+    - intros. auto_under c_x.
+      assert (closed_rty 0 (ctxdom ⦑Γ⦒ ∪ dom aset (<[a:=c_x]> st)) (τ_x ^r^ ({a := c_x }v v2))) as Hclosed.
+      { apply closed_rty_subst_var; auto.
+        apply inv_ctxrR_regular1 in H17; mydestr; eauto.
+        apply ok_dctx_regular in H13; mydestr.
+        apply closed_rty_oarr_implies_closed_rty_retty with (c:=c_x) in H20.
+        refinement_solver. }
+      eapply state_subst_implies_rty_subst_inv_ctxrR_all_open_to_v; eauto.
+      apply inv_ctxrR_regular1 in H17; mydestr; eauto.
+      simpl. eapply IHΓ; eauto; fold value_subst; fold tm_subst.
+      + pose (fv_of_subst_tm a c_x e). set_solver.
+      + refinement_solver.
+      + eapply state_subst_implies_rty_subst_wf_ctxrR_all_v_to_open; eauto.
+      + eapply state_subst_implies_rty_subst_inv_ctxrR_all_v_to_open; eauto.
+        rewrite <- subst_open_var_tm; auto; fast_set_solver.
+   - denotation_simp. apply cons_basic_typing_drop_last_tm.
+      refinement_solver.
+      eapply tletapp_typable with (x:=x); eauto.
+      fast_set_solver. inv_rd_simpl1.
+   - mydestr. auto_meet_exists HE.
+     auto_meet_reduce. dsimp1. rename x5 into c_x. auto_under x0.
+     assert (closed_rty 0 (ctxdom ⦑Γ⦒ ∪ dom aset (<[a:=c_x]> st)) (τ_x ^r^ ({a := c_x }v v2))) as Hclosed.
+      { apply closed_rty_subst_var; auto.
+        apply inv_ctxrR_regular1 in H18; mydestr; eauto.
+        apply closed_rty_oarr_implies_closed_rty_retty with (c:=c_x) in H20.
+        refinement_solver. }
+      eapply state_subst_implies_rty_subst_inv_ctxrR_all_open_to_v; eauto.
+      apply inv_ctxrR_regular1 in H18; mydestr; eauto.
+      simpl. eapply IHΓ; eauto; fold value_subst; fold tm_subst.
+      + pose (fv_of_subst_tm a c_x e). set_solver.
+      + refinement_solver.
+      + eapply state_subst_implies_rty_subst_wf_ctxrR_all_v_to_open; eauto.
+      + eapply state_subst_implies_rty_subst_inv_ctxrR_all_v_to_open; eauto.
+        rewrite <- subst_open_var_tm; auto; fast_set_solver.
+   - denotation_simp. apply cons_basic_typing_drop_last_tm.
+      refinement_solver.
+      eapply tletapp_typable with (x:=x); eauto.
+      fast_set_solver. inv_rd_simpl1.
+   - intros. auto_under v_x.
+     assert (a ∉ stale v2) as Hav.
+     { eapply arr_type_in_tyctx_is_free; eauto; basic_typing_solver. }
+     simpl. rewrite (subst_fresh_value v2); auto.
+     eapply IHΓ; eauto; fold value_subst; fold tm_subst.
+     + pose (fv_of_subst_tm a v_x e).
+       assert (fv_value v_x ≡ ∅). refinement_solver.
+       rewrite H6 in s. set_solver.
+      + simpl in H2. dec_solver2.
+      + rewrite (subst_fresh_tm v2) in H22; auto.
+      + rewrite <- subst_open_var_tm; auto. fast_set_solver. refinement_solver.
+Qed.
+
+Lemma rR_letapp_arr_lam:
+  forall st τ_x e1 (v2: value) τ2,
+    is_arr τ2 ->
+    ({0;b∅;st}⟦τ2⟧) v2 ->
+    ({0;b∅;st}⟦τ2 ⤑ τ_x⟧) (vlam ⌊ τ2 ⌋ e1) ->
+    ({0;b∅;st}⟦ τ_x ⟧) (e1 ^t^ v2).
+Proof.
+  intros; subst. simpl in H0; simpl in H1; mydestr. reduction_simpl0.
+  rewrite closed_rty_destruct_arrarr in H2; mydestr. auto_under v2.
+  eapply termR_perserve_rR; eauto. refinement_solver.
+  apply mk_app_reduce_to_open; refinement_solver.
+Qed.
+
+Lemma rR_letapp_arr_fix:
+  forall st τ_x e1 (v2: value) τ2,
+    is_arr τ2 ->
+    ({0;b∅;st}⟦τ2⟧) v2 ->
+  ({0;b∅;st}⟦τ2 ⤑ τ_x⟧) (vfix (⌊ τ2 ⌋ ⤍ ⌊ τ_x ⌋ ) (vlam ⌊ τ2 ⌋ e1)) ->
+  ({0;b∅;st}⟦ τ_x ⟧) (({1 ~t> v2} e1) ^t^ (vfix (⌊ τ2 ⌋ ⤍ ⌊ τ_x ⌋ ) (vlam ⌊ τ2 ⌋ e1))).
+Proof.
+  intros; subst. simpl in H0; simpl in H1; mydestr. reduction_simpl0.
+  rewrite closed_rty_destruct_arrarr in H2; mydestr. auto_under v2.
+  eapply termR_perserve_rR; eauto. refinement_solver.
+  apply mk_app_reduce_to_open_fix; refinement_solver.
+Qed.
+
+Lemma rR_letapp_arr: forall τ_x τ st x (v1 v2: value) (e: tm) τ2,
+    x ∉ fv_tm e ∪ rty_fv τ ->
+    not_overbasety τ -> not_overbasety τ_x -> is_arr τ2 ->
+    wf_ctxrR st [(x, τ_x)] ->
+    {0;b∅;st}⟦τ2 ⤑ τ_x⟧ v1 ->
+    {0;b∅;st}⟦τ2⟧ v2 ->
+    (⅋{st}⟦τ⟧{[(x, τ_x)] }) (e ^t^ x) ->
+    (⅋{st}⟦τ⟧{[(x, τ_x)] }) (tletapp v1 v2 e).
+Proof.
+  intros.
+  destruct (decide (is_arr τ_x)); intros.
+  - destruct (rR_arrow_value_lam_exists_arrarr _ _ _ _ _ _ H4); mydestr; subst.
+    + rename x0 into e1.
+      assert (({0;b∅;st}⟦τ_x⟧) (e1 ^t^ v2)) as Hz.
+      { eapply rR_letapp_arr_lam in H4; eauto. }
+      pose (rR_arr_halt _ _ _ _ _ i Hz). mydestr.
+      apply wf_implies_ctxrR_tlete_is_arr_better_empty with (x:=x) (e:=e) (τ:=τ) in H7; eauto; try fast_set_solver.
+      eapply termR_perserve_inv_ctxrR; eauto.
+      { invclear H7; refinement_solver. }
+      apply termR_trans_better with (tlete (e1 ^t^ v2) e).
+      simpl. apply termR_weakening. listctx_set_solver.
+      eapply termR_elete_lhs with (x:=x); eauto; try inv_rd_simpl1.
+      apply termR_value_tm; auto; refinement_solver.
+      eapply termR_weakening. listctx_set_solver.
+      simpl. apply termR_tletapp_lam with (Ty := ⌊ τ_x ⌋); auto; inv_rd_simpl1.
+      refinement_solver. refinement_solver.
+      auto_exists_L. intros. inv_rd_simpl1. simpl in H6.
+      assert ( ([] ++ [(x, ⌊τ_x⌋)]) ⊢t e ^t^ x ⋮t ⌊τ⌋) as Hr by auto.
+      apply basic_has_type_renaming with (x0:=y) in Hr. lc_simpl4. fast_set_solver.
+      listctx_set_solver.
+    + rename x0 into e1.
+      assert (({0;b∅;st}⟦τ_x⟧) (({1 ~t> v2} e1) ^t^ (vfix (⌊ τ2 ⌋ ⤍ ⌊τ_x⌋) (vlam ⌊ τ2 ⌋ e1)))) as Hz.
+      { eapply rR_letapp_arr_fix in H4; eauto. }
+      pose (rR_arr_halt _ _ _ _ _ i Hz). mydestr.
+      apply wf_implies_ctxrR_tlete_is_arr_better_empty with (x:=x) (e:=e) (τ:=τ) in H7; eauto; try fast_set_solver.
+      eapply termR_perserve_inv_ctxrR; eauto.
+      { invclear H7; refinement_solver. }
+      apply termR_trans_better with (tlete (({1 ~t> v2} e1) ^t^ (vfix (⌊ τ2 ⌋ ⤍ ⌊τ_x⌋) (vlam ⌊ τ2 ⌋ e1))) e).
+      simpl. apply termR_weakening. listctx_set_solver.
+      eapply termR_elete_lhs with (x:=x); eauto; try inv_rd_simpl1.
+      apply termR_value_tm; auto; refinement_solver.
+      eapply termR_weakening. listctx_set_solver.
+      simpl. apply termR_tletapp_fix; auto; inv_rd_simpl1.
+      refinement_solver. refinement_solver.
+      auto_exists_L. intros. inv_rd_simpl1. simpl in H6.
+      assert ( ([] ++ [(x, ⌊τ_x⌋)]) ⊢t e ^t^ x ⋮t ⌊τ⌋) as Hr by auto.
+      apply basic_has_type_renaming with (x0:=y) in Hr. lc_simpl4. fast_set_solver.
+      listctx_set_solver.
+  - auto_ty_exfalso.
+    destruct (rR_arrow_value_lam_exists_arrarr _ _ _ _ _ _ H4); mydestr; subst.
+    + rename x4 into e1.
+      assert (({0;b∅;st}⟦[v:x0|x1|x2|x3]⟧) (e1 ^t^ v2)) as Hz.
+      { eapply rR_letapp_arr_lam in H4; eauto. }
+      apply wf_implies_ctxrR_tlete_ubase_better_empty with (x:=x) (e:=e) (τ:=τ) in Hz; eauto; try fast_set_solver.
+      eapply termR_perserve_inv_ctxrR; eauto.
+      { invclear Hz; refinement_solver. }
+      apply termR_weakening. listctx_set_solver.
+      apply termR_tletapp_lam with (Ty := x0); eauto.
+      refinement_solver. refinement_solver.
+      auto_exists_L. intros. inv_rd_simpl1. simpl in H6.
+      assert ( ([] ++ [(x, TBase x0)]) ⊢t e ^t^ x ⋮t ⌊τ⌋) as Hr by auto.
+      apply basic_has_type_renaming with (x0:=y) in Hr. lc_simpl4. fast_set_solver.
+      listctx_set_solver.
+    + rename x4 into e1.
+      assert (({0;b∅;st}⟦[v:x0|x1|x2|x3]⟧) (({1 ~t> v2} e1) ^t^ (vfix (⌊ τ2 ⌋ ⤍ x0) (vlam ⌊ τ2 ⌋ e1)))) as Hz.
+      { eapply rR_letapp_arr_fix in H4; eauto. }
+      apply wf_implies_ctxrR_tlete_ubase_better_empty with (x:=x) (e:=e) (τ:=τ) in Hz; eauto; try fast_set_solver.
+      eapply termR_perserve_inv_ctxrR; eauto.
+      { invclear Hz; refinement_solver. }
+      apply termR_weakening. listctx_set_solver.
+      apply termR_tletapp_fix; eauto.
+      refinement_solver. refinement_solver.
+      auto_exists_L. intros. inv_rd_simpl1. simpl in H6.
+      assert ( ([] ++ [(x, TBase x0)]) ⊢t e ^t^ x ⋮t ⌊τ⌋) as Hr by auto.
+      apply basic_has_type_renaming with (x0:=y) in Hr. lc_simpl4. fast_set_solver.
+      listctx_set_solver.
+Qed.
+
+Lemma inv_rRctx_letapp_arrarr: forall Γ st (τ: rty) x τ2 τ_x (v1 v2: value) e,
+    x ∉ fv_tm e ∪ rty_fv τ -> not_overbasety τ -> not_overbasety τ_x -> is_arr τ2 ->
+    closed_rty 0 (ctxdom ⦑Γ⦒ ∪ dom aset st) τ ->
+    wf_ctxrR st (Γ ++ [(x, τ_x)]) ->
+    (⅋{st}⟦τ2 ⤑ τ_x⟧{Γ}) v1 ->
+    (⅋{st}⟦τ2⟧{Γ}) v2 ->
+    (⅋{st}⟦τ⟧{Γ ++ [(x, τ_x)] }) (e ^t^ x) ->
+    ⅋{st}⟦τ⟧{Γ ++ [(x, τ_x)] } (tletapp v1 v2 e).
+Proof.
+  induction Γ; intros. listctx_set_simpl. invclear H5. invclear H6. eapply rR_letapp_arr; eauto.
+  mydestr. assert (a ∉ dom aset st ∪ ctxdom Γ ∪ {[x]}) as Ha.
+  { RD_simp2; refinement_solver. }
+  assert (((a, ⌊ r ⌋) :: ⌊Γ ++ [(x, τ_x)]⌋*) ⊢t tletapp v1 v2 e ⋮t ⌊τ⌋) as HT.
+          { denotation_simp.
+            apply cons_basic_typing_drop_last_tm.
+            apply inv_ctxrR_regular in H7; mydestr. refinement_solver.
+            inv_rd_simpl1. inv_rd_simpl3.
+            eapply tletapp_typable with (x:=x); eauto.
+            fast_set_solver. inv_rd_simpl1. }
+  RD_simp2; constructor; auto.
+    - intros. auto_under c_x.
+      eapply IHΓ; eauto; fold value_subst; fold tm_subst.
+      + pose (fv_of_subst_tm a c_x e). set_solver.
+      + refinement_solver.
+      + rewrite <- subst_open_var_tm; auto. fast_set_solver.
+   - mydestr. auto_meet_exists HE.
+     auto_meet_reduce. dsimp1. rename x4 into c_x. auto_under x0.
+     eapply IHΓ; eauto; fold value_subst; fold tm_subst.
+      + pose (fv_of_subst_tm a c_x e). set_solver.
+      + refinement_solver.
+      + rewrite <- subst_open_var_tm; auto; fast_set_solver.
+   - intros. auto_under v_x.
+     apply IHΓ with (τ2 := τ2); eauto; fold value_subst; fold tm_subst.
+     + pose (fv_of_subst_tm a v_x e).
+       assert (fv_value v_x ≡ ∅). refinement_solver.
+       rewrite H6 in s. set_solver.
+      + simpl in H3. dec_solver2.
+      + rewrite <- subst_open_var_tm; auto. fast_set_solver. refinement_solver.
+Qed.
+
+Ltac auto_dclosed_rty:=
+  repeat match goal with
+    | [H: closed_rty _ _ (-:{v: _ | _ | _ | _}⤑ _) |- _ ] => rewrite closed_rty_destruct_oarr in H; mydestr; auto
+    | [H: closed_rty _ _ (_ ⤑ _) |- _ ] => rewrite closed_rty_destruct_arrarr in H; mydestr; auto
+    | [|- closed_rty _ _ (-:{v: _ | _ | _ | _}⤑ _) ] => rewrite closed_rty_destruct_oarr; split; auto
+    | [|- closed_rty _ _ (_ ⤑ _)] => rewrite closed_rty_destruct_arrarr; mydestr; split; auto
+    end.
+
+Lemma well_founded_phi_implies_lt: forall st (c c': constant) (ϕ: refinement),
+    ϕ b∅ st c -> (≻≻ ϕ) (<b[↦c]> b∅) st c' -> c ≻ c'.
+Proof.
+  unfold well_founded_constraint. intros. mydestr. auto.
+Qed.
+
+Lemma well_founded_phi_implies_phi: forall st bst (c: constant) (ϕ: refinement),
+    (≻≻ ϕ) bst st c -> ϕ bst st c.
+Proof.
+  unfold well_founded_constraint. intros. mydestr. auto.
+Qed.
+
+Lemma closed_obase_implies_all_bst: forall b n d ϕ (L: aset),
+    closed_rty 0 L {v:b|n|d|ϕ} -> (forall st bst1 bst2 c, ϕ bst1 st c <-> ϕ bst2 st c).
+Proof.
+  intros. apply bound_in_refinement_0. refinement_solver. invclear H0. invclear H5. auto.
+Qed.
+
+Lemma closed_rty_implies_bound_plus1: forall τ m (L:aset),
+    closed_rty m L τ -> closed_rty (S m) L τ.
+Proof.
+  induction τ; intros; auto.
+  - invclear H; constructor; auto. invclear H1. constructor; auto.
+  - invclear H; constructor; auto. invclear H1. constructor; auto.
+  - auto_dclosed_rty. invclear H; constructor; auto. invclear H3. constructor; auto.
+  - auto_dclosed_rty.
+Qed.
+
+Global Hint Resolve closed_rty_implies_bound_plus1: core.
+
+Lemma rR_implies_bound_plus1: forall τ m bst st e,
+    ({m;bst;st}⟦τ⟧) e <-> ({S m;bst;st}⟦τ⟧ e /\ closed_rty m (dom aset st) τ).
+Proof.
+  induction τ; split; intros; auto; simpl in H; mydestr; subst.
+  - do 3 (constructor; eauto).
+  - constructor; eauto.
+  - do 3 (constructor; eauto).
+  - constructor; eauto.
+  - do 3 (constructor; eauto). eexists; split; eauto. intros.
+    apply H2 in H4; auto. rewrite IHτ in H4; mydestr; auto.
+  - do 2 (constructor; eauto). eexists; split; eauto. intros.
+    apply H3 in H5; auto. auto_dclosed_rty. rewrite IHτ; split; auto.
+  - do 3 (constructor; eauto). eexists; split; eauto. intros.
+    auto_dclosed_rty.
+    assert (({S m;bst;st}⟦τ1⟧) v_x /\ closed_rty m (dom aset st) τ1) as Hz by auto.
+    rewrite <- IHτ1 in Hz. auto_under v_x. rewrite IHτ2 in H2; mydestr; auto.
+  - do 2 (constructor; eauto). eexists; split; eauto. intros.
+    auto_dclosed_rty. rewrite IHτ1 in H4. mydestr. auto_under v_x.
+    rewrite IHτ2. split; auto.
+Qed.
+
+Lemma fix_rR_aux_c: forall st b n d ϕ τ e,
+    [] ⊢t vfix (TBase b ⤍ ⌊τ⌋) (vlam b e) ⋮v (TBase b ⤍ ⌊τ⌋) ->
+    closed_rty 0 (dom aset st) (-:{v: b | n | d | ϕ}⤑ τ) ->
+    forall (c: constant),
+    {0;b∅;st}⟦{v: b | n | d | ϕ}⟧ c ->
+    (forall (c_x: constant),
+        {0;b∅;st}⟦{v: b | n | d | ϕ}⟧ c_x ->
+        ({1;<b[↦c_x]> b∅;st}⟦(-:{v: b | S n | d | ≻≻ ϕ}⤑ τ) ⤑ τ⟧) ((vlam (b ⤍ ⌊τ⌋) e) ^t^ c_x)) ->
+    ({1;<b[↦c]> b∅;st}⟦τ⟧) (({1 ~t> c} e) ^t^ (vfix (b ⤍ ⌊τ⌋) (vlam b e))).
+Proof.
+  intros st b n d ϕ τ e HTfix Hclosed.
+  apply (well_founded_induction_type well_founded_R_constant_is_well_founded
+           (fun c =>
+                {0;b∅;st}⟦{v: b | n | d | ϕ}⟧ c ->
+                (forall (c_x: constant),
+                    {0;b∅;st}⟦{v: b | n | d | ϕ}⟧ c_x ->
+                    ({1;<b[↦c_x]> b∅;st}⟦(-:{v: b | S n | d | ≻≻ ϕ}⤑ τ) ⤑ τ⟧) ((vlam (b ⤍ ⌊τ⌋) e) ^t^ c_x)) ->
+                ({1;<b[↦c]> b∅;st}⟦τ⟧) (({1 ~t> c} e) ^t^ (vfix (b ⤍ ⌊τ⌋) (vlam b e))))
+        ).
+  intros c; intros.
+  assert (({1;<b[↦c]> b∅;st}⟦(-:{v: b | S n | d | ≻≻ ϕ}⤑ τ) ⤑ τ⟧)
+             (vlam (b ⤍ ⌊τ⌋) e ^t^ c)) as Hz; auto.
+  destruct Hz. destruct H3. do 2 destruct H4. simpl in H4.
+  assert (x = (vlam (b ⤍ ⌊τ⌋) ({1 ~t> c }e))) by (reduction_simpl1; auto); subst. clear H4.
+  assert (({1;<b[↦c]> b∅;st}⟦-:{v: b | S n | d | ≻≻ ϕ}⤑ τ⟧) (vfix (b ⤍ ⌊τ⌋) (vlam b e))).
+  - constructor; auto. constructor; auto. auto_dclosed_rty.
+    exists (vfix (b ⤍ ⌊τ⌋) (vlam b e)). split; eauto. apply multistep_refl. basic_typing_solver.
+    intros c'. intros.
+    assert (c ≻ c').
+    { eapply well_founded_phi_implies_lt; eauto.
+      simpl in H0; mydestr; subst. invclear H10. auto. }
+    assert (({1;<b[↦c']> b∅;st}⟦τ⟧) (mk_app (vfix (b ⤍ ⌊τ⌋) (vlam b e)) c')).
+    eapply termR_perserve_rR; auto. refinement_solver. refinement_solver.
+    apply mk_app_reduce_to_open_fix'; auto.
+    eapply H; eauto.
+    + constructor; auto. constructor; auto. auto_dclosed_rty.
+      exists c'. split; auto. split; auto. apply well_founded_phi_implies_phi in H6.
+      auto_dclosed_rty. rewrite closed_obase_implies_all_bst in H6; eauto.
+    + rewrite rR_bst_bound in H8; eauto.
+      rewrite rR_implies_bound_plus1 in H8; mydestr; eauto.
+      unfold bst_eq. unfold bstate_push. intros.
+      destruct i; auto. destruct i; auto. lia.
+  - auto_under (vfix (b ⤍ ⌊τ⌋) (vlam b e)).
+    apply termR_perserve_rR with (e':=({1 ~t> c} e) ^t^ (vfix (b ⤍ ⌊τ⌋) (vlam b e))) in H5; auto.
+    refinement_solver. refinement_solver.
+    apply mk_app_reduce_to_open; auto.
+    eapply vfix_implies_open_tyable with (v2:=c) in HTfix; eauto.
+    refinement_solver.
+Qed.
+
+Lemma fix_rR: forall τ st b n d ϕ e,
+    closed_rty 0 (dom aset st) (-:{v: b | n | d | ϕ}⤑ τ) ->
+    {0;b∅;st}⟦-:{v: b | n | d | ϕ}⤑ (-:{v: b | S n | d | ≻≻ ϕ}⤑ τ) ⤑ τ⟧ (vlam b (vlam (b ⤍ ⌊τ⌋) e)) ->
+    {0;b∅;st}⟦-:{v: b | n | d | ϕ}⤑ τ⟧ (vfix (b ⤍ ⌊τ⌋) (vlam b e)).
+Proof.
+  intros. destruct H0. destruct H1. do 2 destruct H2.
+  assert ([] ⊢t vfix (b ⤍ ⌊τ⌋) (vlam b e) ⋮t b ⤍ ⌊τ⌋) as HT.
+  { basic_typing_solver. invclear H6.
+    auto_exists_L. intros; eauto.
+    assert (f ∉ L) by fast_set_solver. apply H5 in H4. invclear H4; auto. }
+  assert (x = vlam b (vlam (b ⤍ ⌊τ⌋) e)) by (reduction_simpl1; auto); subst. clear H2.
+  do 2 (constructor; auto).
+  exists (vfix (b ⤍ ⌊τ⌋) (vlam b e)). split; eauto. apply multistep_refl. basic_typing_solver.
+  intros. auto_dclosed_rty.
+  eapply termR_perserve_rR; auto. refinement_solver.
+  apply mk_app_reduce_to_open_fix'; auto. basic_typing_solver.
+  apply fix_rR_aux_c with (n:=n) (d:=d) (ϕ:=ϕ); eauto.
+  - basic_typing_solver.
+  - auto_dclosed_rty.
+  - do 2 (constructor; eauto).
+  - intros. simpl in H14; mydestr; subst. invclear H18.
+    apply H3 in H17; auto.
+    eapply termR_perserve_rR; eauto. refinement_solver.
+    apply mk_app_reduce_to_open; auto. inv_rd_simpl1.
+Qed.
+
+Lemma wf_ctxrR_implies_fix: forall Γ st b d ϕ τ e,
+  wf_ctxrR st Γ ->
+  closed_rty 0 (ctxdom ⦑Γ⦒ ∪ dom aset st) (-:{v: b | 0 | d | ϕ}⤑ τ) ->
+  (⅋{st}⟦-:{v: b | 0 | d | ϕ}⤑ (-:{v: b | 1 | d | ≻≻ ϕ}⤑ τ) ⤑ τ⟧{Γ}) (vlam b (vlam (b ⤍ ⌊τ⌋) e)) ->
+  (⅋{st}⟦-:{v: b | 0 | d | ϕ}⤑ τ⟧{Γ}) (vfix (b ⤍ ⌊τ⌋) (vlam b e)).
+Proof.
+  induction Γ; intros. RD_simp2. apply fix_rR; auto. closed_rty_solver.
+  mydestr.
+  assert (((a, ⌊r⌋) :: ⌊Γ⌋*) ⊢t vfix (b ⤍ ⌊τ⌋) (vlam b e) ⋮t ⌊-:{v: b | 0 | d | ϕ}⤑ τ⌋) as HT.
+          { apply inv_ctxrR_regular in H1; mydestr.
+            basic_typing_solver. invclear H7.
+            auto_exists_L. intros; eauto.
+            assert (f ∉ L) by fast_set_solver. apply H6 in H5. invclear H5; auto.
+          }
+          RD_simp2.
+  - constructor; auto.
+    intros. auto_under c_x. simpl.
+    apply IHΓ; auto. closed_rty_solver.
+  - constructor; auto.
+    mydestr. auto_meet_exists Hmeet. auto_meet_reduce.
+    simpl. apply IHΓ; eauto; dsimp1. closed_rty_solver.
+  - constructor; auto. inv_rd_simpl1.
+    intros. auto_under v_x. simpl.
+    apply IHΓ; auto. inv_rd_simpl1.
+Qed.
